disk-betree/ImplModelCache.i.dfy
@@ -1,0 +1,64 @@
+include "ImplModel.i.dfy"
+include "../lib/Sets.i.dfy"
+
+module ImplModelCache { 
+  import opened ImplModel
+
+  import opened Options
+  import opened Maps
+  import opened Sequences
+  import opened Sets
+
+  import opened NativeTypes
+
+  predicate RefAvailable(s: Variables, ref: Reference)
+  {
+    && s.Ready?
+    && ref !in s.ephemeralIndirectionTable
+    && ref !in s.cache 
+  }
+
+  function getFreeRefIterate(s: Variables, i: uint64) 
+  : (ref : Option<BT.G.Reference>)
+  requires s.Ready?
+  ensures ref.Some? ==> RefAvailable(s, ref.value)
+  decreases 0x1_0000_0000_0000_0000 - i as int
+  {
+    if i !in s.ephemeralIndirectionTable && i !in s.cache then (
+      Some(i)
+    ) else if i == 0xffff_ffff_ffff_ffff then (
+      None
+    ) else (
+      getFreeRefIterate(s, i+1) 
+    )
+  }
+
+  function {:opaque} getFreeRef(s: Variables)
+  : (ref : Option<BT.G.Reference>)
+  requires s.Ready?
+  ensures ref.Some? ==> RefAvailable(s, ref.value)
+  {
+    getFreeRefIterate(s, 0)
+  }
+
+  function {:opaque} write(k: Constants, s: Variables, ref: BT.G.Reference, node: Node)
+  : (s': Variables)
+  requires s.Ready?
+  {
+    // TODO how do we deal with this?
+    var eph := s.ephemeralIndirectionTable[ref := (None, if node.children.Some? then node.children.value else [])];
+    s.(ephemeralIndirectionTable := eph).(cache := s.cache[ref := node])
+  }
+
+  function {:opaque} alloc(k: Constants, s: Variables, node: Node)
+  : (p: (Variables, Option<Reference>))
+  requires s.Ready?
+  {
+    var ref := getFreeRef(s);
+    if ref.Some? then (
+      (write(k, s, ref.value, node), ref)
+    ) else (
+      (s, None)
+    )
+  }
+}
