disk-betree/ImplModelFlush.i.dfy
@@ -1,0 +1,75 @@
+include "ImplModelCache.i.dfy"
+include "AsyncDiskModel.s.dfy"
+
+module ImplModelFlush { 
+  import opened ImplModel
+  import opened ImplModelCache
+
+  import opened Options
+  import opened Maps
+  import opened Sequences
+  import opened Sets
+
+  import opened BucketsLib
+
+  import opened NativeTypes
+  import D = AsyncDisk
+
+  function flush(k: Constants, s: Variables, parentref: BT.G.Reference, slot: int)
+  : (Variables, DiskOp)
+  requires Inv(k, s)
+  requires s.Ready?
+  requires parentref in s.ephemeralIndirectionTable
+  requires parentref in s.cache
+  requires s.cache[parentref].children.Some?
+  requires 0 <= slot < |s.cache[parentref].buckets|
+  requires s.rootBucket == map[] // FIXME we don't actually need this unless we're flushing the root
+  {
+    if (
+      && s.frozenIndirectionTable.Some?
+      && parentref in s.frozenIndirectionTable.value
+      && var entry := s.frozenIndirectionTable.value[parentref];
+      && var (loc, _) := entry;
+      && loc.None?
+    ) then (
+      (s, D.NoDiskOp)
+    ) else (
+      var node := s.cache[parentref];
+      var childref := node.children.value[slot];
+      if (childref !in s.cache) then (
+        PageInReq(k, s, io, childref)
+      ) else (
+        var child := s.cache[childref];
+        if (!(
+          && |node.buckets[slot].keys| < 0x4000_0000_0000_0000
+          && |child.buckets| < 0x1_0000_0000_0000_0000
+          && (forall i | 0 <= i < |child.buckets| :: |child.buckets[i].keys| < 0x4000_0000_0000_0000)
+        )) then (
+          (s, NoDiskOp)
+        ) else (
+          var newbuckets := KMTable.Flush(node.buckets[slot], child.buckets, child.pivotTable);
+          var newchild := child.(buckets := newbuckets);
+          var s1, newchildref := alloc(k, s, newchild);
+          if newchildref.None? then (
+            (s1, NoDiskOp)
+          ) else (
+            var newparent := Node(
+              node.pivotTable,
+              Some(node.children.value[slot := newchildref.value]),
+              node.buckets[slot := KMTable.Empty()]
+            );
+            var s' := write(k, s1, parentref, newparent);
+            s'
+          )
+        )
+      )
+    )
+  }
+
+  lemma flushCorrect(k: Constants, s: Variables, parentref: BT.G.Reference, slot: int)
+  requires flush.requires(k, s, parentref, slot)
+  ensures
+      var (s', diskOp) := flush(k, s, parentref, slot);
+      && WFVars(s')
+      && ImplADM.M.Next(Ik(k), I(k, s), I(k, s'), UI.NoOp, diskOp)
+}
